{
 "cells": [
  {
   "cell_type": "markdown",
   "id": "a69a79fc-e535-4d7e-92f0-f19c8d60e349",
   "metadata": {},
   "source": [
    "$\\textbf{Assignment - PreMidterms}$\n",
    "-"
   ]
  },
  {
   "cell_type": "markdown",
   "id": "0a1e42d1-4cad-4097-b5b2-398a08e85391",
   "metadata": {},
   "source": [
    "$\\textbf{1.}$\n",
    "Recall the definition of a rational number, denoted as $\\mathbb{Q}$. Prove that the Euler's number $e = \\Sigma_{k=0}^\\infty \\frac{1}{k!} \\notin \\mathbb{Q}$. A factorial is defined as $k! = (k)(k-1)(k-2)(k-3)..., \\forall k \\in \\mathbb{Z}^+$, note that $0! = 1$. Furthermore, a sum notation\n",
    "$\\Sigma_{k=0}^\\infty k = 0+ 1 + 2 + 3 +....+...$\n",
    "\n",
    "$\\textbf{Solution: }$\n",
    "--\n",
    "\n",
    "To prove that Euler's number $ e $ is not a rational number, we can use the fact that if a number is rational, it can be expressed as a fraction of two integers where the denominator is not zero.\n",
    "\n",
    "Let's assume $ e $ is rational. Then it can be written as $ e = \\frac{a}{b} $, where $ a $ and $ b $ are integers with no common factors other than $ 1 $, and $ b \\neq 0 $.\n",
    "\n",
    "Now, let's consider the series expansion of $ e $:\n",
    "\n",
    "$$\n",
    "e = \\sum_{k=0}^{\\infty} \\frac{1}{k!} = 1 + \\frac{1}{1!} + \\frac{1}{2!} + \\frac{1}{3!} + \\cdots\n",
    "$$\n",
    "\n",
    "For any integer $ n $, let's consider the partial sum $ S_n $:\n",
    "\n",
    "$$\n",
    "S_n = 1 + \\frac{1}{1!} + \\frac{1}{2!} + \\frac{1}{3!} + \\cdots + \\frac{1}{n!}\n",
    "$$\n",
    "\n",
    "Since $ S_n $ is a finite sum of rational numbers, it is also rational.\n",
    "\n",
    "Now, let's consider the difference $ e - S_n $:\n",
    "\n",
    "$$\n",
    "e - S_n = \\left(\\sum_{k=0}^{\\infty} \\frac{1}{k!}\\right) - \\left(\\sum_{k=0}^{n} \\frac{1}{k!}\\right) = \\frac{1}{(n+1)!} + \\frac{1}{(n+2)!} + \\frac{1}{(n+3)!} + \\cdots\n",
    "$$\n",
    "\n",
    "Each term in this series is positive and less than $ \\frac{1}{(n+1)!} $. Therefore, $ e - S_n $ is positive and less than $ \\frac{1}{(n+1)!} $.\n",
    "\n",
    "Now, consider $ b! $ where $ b $ is some integer greater than $ n $. We can express $ b! $ as:\n",
    "\n",
    "$$\n",
    "b! = (n+1)! \\cdot (n+2) \\cdot (n+3) \\cdot \\cdots \\cdot b\n",
    "$$\n",
    "\n",
    "Since $ b > n $, all terms in the product are greater than or equal to $ 2 $. Therefore, $ b! $ is divisible by $ (n+1)! $.\n",
    "\n",
    "This implies that $ e - S_n $ is less than $ \\frac{1}{b!} $.\n",
    "\n",
    "However, since $ e = \\frac{a}{b} $, $ e - S_n $ can also be written as a fraction with denominator $ b $.\n",
    "\n",
    "But we've just shown that $ e - S_n $ is less than $ \\frac{1}{b!} $, which implies that $ e - S_n $ is less than $ \\frac{1}{b} $.\n",
    "\n",
    "This contradicts the fact that $ e - S_n $ is a positive number less than $ \\frac{1}{b!} $.\n",
    "\n",
    "Therefore, our assumption that $ e $ is rational"
   ]
  },
  {
   "cell_type": "markdown",
   "id": "74eb78e7-4580-4b60-8d38-fdd5b9cf6a5e",
   "metadata": {},
   "source": [
    "$\\textbf{2.}$\n",
    "Prove Minkowski's Inequality for sums, $\\forall \\ p>1, (a_k, b_k)>0$:\n",
    "\\begin{gather}\n",
    "\\begin{bmatrix}\n",
    "\\Sigma_{k=1}^n |a_k + b_k|^p\n",
    "\\end{bmatrix}^\\frac{1}{p}\n",
    "\\leq\n",
    "\\begin{bmatrix}\n",
    "\\Sigma_{k=1}^n |a_k|^p\n",
    "\\end{bmatrix}^\\frac{1}{p}\n",
    "+\n",
    "\\begin{bmatrix}\n",
    "\\Sigma_{k=1}^n |b_k|^p\n",
    "\\end{bmatrix}^\\frac{1}{p}\n",
    "\\end{gather}\n",
    "\n",
    "$\\textbf{Solution:}$\n",
    "--\n",
    "\n",
    "To prove Minkowski's inequality for sums, we first need to establish Holder's inequality. Holder's inequality states that for any sequences of real numbers $ (a_k) $ and $ (b_k) $ and any $ p > 1 $ such that $ \\frac{1}{p} + \\frac{1}{q} = 1 $, we have:\n",
    "\n",
    "$$\n",
    "\\sum_{k=1}^n |a_k b_k| \\leq \\left( \\sum_{k=1}^n |a_k|^p \\right)^{\\frac{1}{p}} \\left( \\sum_{k=1}^n |b_k|^q \\right)^{\\frac{1}{q}}\n",
    "$$\n",
    "\n",
    "where $ q $ is the conjugate exponent of $ p $, i.e., $ q = \\frac{p}{p-1} $.\n",
    "\n",
    "Now, let's use Holder's inequality to prove Minkowski's inequality. We'll set $ b_k = 1 $ for all $ k $ and apply Holder's inequality:\n",
    "\n",
    "$$\n",
    "\\sum_{k=1}^n |a_k + 1|^p \\leq \\left( \\sum_{k=1}^n |a_k|^p \\right)^{\\frac{1}{p}} \\left( \\sum_{k=1}^n |1|^q \\right)^{\\frac{1}{q}} = \\left( \\sum_{k=1}^n |a_k|^p \\right)^{\\frac{1}{p}} \\left( \\sum_{k=1}^n 1 \\right)^{\\frac{1}{q}}\n",
    "$$\n",
    "\n",
    "Now, $ \\sum_{k=1}^n 1 = n $, so:\n",
    "\n",
    "$$\n",
    "\\left( \\sum_{k=1}^n |a_k + 1|^p \\right)^{\\frac{1}{p}} \\leq \\left( \\sum_{k=1}^n |a_k|^p \\right)^{\\frac{1}{p}} \\cdot n^{\\frac{1}{q}}\n",
    "$$\n",
    "\n",
    "Since $ q = \\frac{p}{p-1} $, $ \\frac{1}{q} = \\frac{p-1}{p} $. So, $ n^{\\frac{1}{q}} = n^{\\frac{p-1}{p}} $.\n",
    "\n",
    "Substituting back into the inequality, we get:\n",
    "\n",
    "$$\n",
    "\\left( \\sum_{k=1}^n |a_k + 1|^p \\right)^{\\frac{1}{p}} \\leq \\left( \\sum_{k=1}^n |a_k|^p \\right)^{\\frac{1}{p}} \\cdot n^{\\frac{p-1}{p}}\n",
    "$$\n",
    "\n",
    "Now, since $ n^{\\frac{p-1}{p}} = \\sqrt[p]{n^{p-1}} $, we can rewrite it as $ n^{\\frac{1}{p}} $. Therefore:\n",
    "\n",
    "$$\n",
    "\\left( \\sum_{k=1}^n |a_k + 1|^p \\right)^{\\frac{1}{p}} \\leq \\left( \\sum_{k=1}^n |a_k|^p \\right)^{\\frac{1}{p}} \\cdot n^{\\frac{1}{p}}\n",
    "$$\n",
    "\n",
    "This is equivalent to:\n",
    "\n",
    "$$\n",
    "\\left( \\sum_{k=1}^n |a_k + 1|^p \\right)^{\\frac{1}{p}} \\leq \\left( \\sum_{k=1}^n |a_k|^p \\right)^{\\frac{1}{p}} + n^{\\frac{1}{p}}\n",
    "$$\n",
    "\n",
    "which is the desired Minkowski's inequality for sums.desired Minkowski's inequality for sums."
   ]
  },
  {
   "cell_type": "markdown",
   "id": "81394dd6-acf8-4737-8cb1-590d6250073e",
   "metadata": {},
   "source": [
    "$\\textbf{3.}$\n",
    "Prove the triangle inequality $|x+y| \\leq |x| + |y|, \\forall (x,y) \\in \\mathbb{R}$\n",
    "\n",
    "$\\textbf{Solution:}$\n",
    "--\n",
    "\n",
    "To prove the triangle inequality $ |x+y| \\leq |x| + |y|, \\forall (x,y) \\in \\mathbb{R} $:\n",
    "\n",
    "We can start by considering two cases: \n",
    "\n",
    "1. When $x \\geq 0$ and $y \\geq 0$: In this case, $|x+y| = x + y$. Since $x$ and $y$ are both non-negative, it follows that $|x| = x$ and $|y| = y$. Therefore, the inequality reduces to $x + y \\leq x + y$, which is obviously true.\n",
    "\n",
    "2. When $x < 0$ or $y < 0$: Without loss of generality, let's assume $x < 0$. Then $|x| = -x$ and $|y| = -y$. Now, $|x+y| = -(x+y)$. By distributing the negative sign, we get $|x+y| = -x - y$. Now, $|x| + |y| = -x - y$. \n",
    "\n",
    "In this case, $|x+y| = -(x+y)$, and $|x| + |y| = -x - y$. Since $-(x+y) = -x - y$, the inequality holds true in this case as well.\n",
    "\n",
    "Therefore, in all cases, $|x+y| \\leq |x| + |y|, \\forall (x,y) \\in \\mathbb{R}$."
   ]
  },
  {
   "cell_type": "markdown",
   "id": "8595fc9f-45c8-4446-894c-392d22a301c0",
   "metadata": {},
   "source": [
    "$\\textbf{4.}$\n",
    "Prove Sedrakayan's Lemma $\\forall u_i, v_i \\in \\mathbb{R}^+$:\n",
    "\\begin{gather}\n",
    "\\frac{(\\Sigma_{i=1}^n u_i)^2}{\\Sigma_{i=1}^n v_i}\n",
    "\\leq\n",
    "\\Sigma_{i=1}^n \\frac{(u_i)^2}{v_i}\n",
    "\\end{gather}\n",
    "\n",
    "$\\textbf{Solution:}$\n",
    "--\n",
    "\n",
    "To prove Sedrakyan's Lemma $ \\forall u_i, v_i \\in \\mathbb{R}^+ $:\n",
    "\n",
    "Let's start by expanding the terms on both sides of the inequality:\n",
    "\n",
    "Left-hand side (LHS):\n",
    "$$\n",
    "\\frac{(\\sum_{i=1}^n u_i)^2}{\\sum_{i=1}^n v_i} = \\frac{(\\sum_{i=1}^n u_i)(\\sum_{i=1}^n u_i)}{\\sum_{i=1}^n v_i}\n",
    "$$\n",
    "\n",
    "Right-hand side (RHS):\n",
    "$$\n",
    "\\sum_{i=1}^n \\frac{u_i^2}{v_i}\n",
    "$$\n",
    "\n",
    "Now, consider the expansion of the product $ (\\sum_{i=1}^n u_i)(\\sum_{i=1}^n u_i) $ in the numerator of the LHS:\n",
    "\n",
    "$$\n",
    "(\\sum_{i=1}^n u_i)(\\sum_{i=1}^n u_i) = \\sum_{i=1}^n \\sum_{j=1}^n u_i u_j\n",
    "$$\n",
    "\n",
    "Expanding the terms, we have:\n",
    "$$\n",
    "\\sum_{i=1}^n \\sum_{j=1}^n u_i u_j = \\sum_{i=1}^n u_i^2 + 2\\sum_{1 \\leq i < j \\leq n} u_i u_j\n",
    "$$\n",
    "\n",
    "Now, since $ u_i, v_i > 0 $, we know that $ u_i^2 \\geq 0 $ and $ u_i u_j \\geq 0 $ for all $ i, j $. Therefore, each term in the expansion of the LHS is non-negative.\n",
    "\n",
    "Now, let's compare the terms of the LHS and RHS:\n",
    "\n",
    "1. The term $ \\sum_{i=1}^n u_i^2 $ appears in both the LHS and RHS.\n",
    "2. The term $ 2\\sum_{1 \\leq i < j \\leq n} u_i u_j $ appears only in the expansion of the LHS.\n",
    "\n",
    "Since all terms in the expansion of the LHS are non-negative, and the expansion of the LHS contains additional terms compared to the RHS, we can conclude that:\n",
    "$$\n",
    "\\frac{(\\sum_{i=1}^n u_i)^2}{\\sum_{i=1}^n v_i} \\leq \\sum_{i=1}^n \\frac{u_i^2}{v_i}\n",
    "$$\n",
    "\n",
    "This proves Sedrakyan's Lemma.\""
   ]
  },
  {
   "cell_type": "markdown",
   "id": "6776c2df-016d-4684-934f-81c7913aeb8d",
   "metadata": {},
   "source": [
    "1. Consider the functions $f(x) = 2x+1$, $g(x)=2y-1$, $j(x) = |f(x)+g(x)|$, and $h(x) = j(x)^2$, show for the following inequality that:\n",
    "\n",
    "\\begin{gather}\n",
    "\\sqrt{|f(x)|^2} \\geq \\sqrt{h(x)} - \\sqrt{|g(x)|^2}, \\forall (x,y) \\in \\mathbb{Z}^+\n",
    "\\end{gather}\n",
    "\n",
    "$\\textbf{Solution:}$\n",
    "--\n",
    "\n",
    "Now, let's evaluate each term:\n",
    "\n",
    "1. $|f(x)|^2 = (2x+1)^2$\n",
    "2. $|g(x)|^2 = (2y-1)^2$\n",
    "3. $h(x) = j(x)^2 = |f(x) + g(x)|^2 = |(2x+1) + (2y-1)|^2 = |2x + 2y|^2 = (2x + 2y)^2$\n",
    "\n",
    "Now, substitute these expressions into the inequality:\n",
    "\n",
    "$$\n",
    "\\sqrt{(2x+1)^2} \\geq \\sqrt{(2x + 2y)^2} - \\sqrt{(2y-1)^2}\n",
    "$$\n",
    "\n",
    "This simplifies to:\n",
    "\n",
    "$$\n",
    "|2x+1| \\geq |2x + 2y| - |2y-1|\n",
    "$$\n",
    "\n",
    "Since $|2x+1| = |2x + 2y| - |2y-1|$ holds true for all positive integers $x$ and $y$, the inequality is verified."
   ]
  },
  {
   "cell_type": "markdown",
   "id": "8e23a4ca-7256-48d2-8fb6-0bafce91162d",
   "metadata": {},
   "source": [
    "2. Prove Sedrakayan's Lemma if $u_i, v_i$ are square roots of an even integers:\n",
    "\\begin{gather}\n",
    "\\frac{(\\Sigma_{i=1}^n u_i)^2}{\\Sigma_{i=1}^n v_i}\n",
    "\\leq\n",
    "\\Sigma_{i=1}^n \\frac{(u_i)^2}{v_i}\n",
    "\\end{gather}\n",
    "\n",
    "$\\textbf{Solution:}$\n",
    "--\n",
    "\n",
    "To prove Sedrakayan's Lemma when $ u_i $ and $ v_i $ are square roots of even integers:\n",
    "\n",
    "Let $ u_i = \\sqrt{2a_i} $ and $ v_i = \\sqrt{2b_i} $, where $ a_i $ and $ b_i $ are positive integers. We need to show:\n",
    "\n",
    "$$\n",
    "\\frac{\\left( \\sum_{i=1}^n \\sqrt{2a_i} \\right)^2}{\\sum_{i=1}^n \\sqrt{2b_i}} \\leq \\sum_{i=1}^n \\frac{(2a_i)}{(2b_i)}\n",
    "$$\n",
    "\n",
    "Expanding the terms, we get:\n",
    "\n",
    "$$\n",
    "\\frac{\\left( \\sum_{i=1}^n \\sqrt{2a_i} \\right)^2}{\\sum_{i=1}^n \\sqrt{2b_i}} = \\frac{\\left( \\sum_{i=1}^n \\sqrt{2a_i} \\right) \\left( \\sum_{i=1}^n \\sqrt{2a_i} \\right)}{\\sum_{i=1}^n \\sqrt{2b_i}}\n",
    "$$\n",
    "\n",
    "and\n",
    "\n",
    "$$\n",
    "\\sum_{i=1}^n \\frac{(2a_i)}{(2b_i)} = \\sum_{i=1}^n \\frac{2a_i}{2b_i}\n",
    "$$\n",
    "\n",
    "Since $ \\sqrt{2a_i} $ and $ \\sqrt{2b_i} $ are positive, we can rewrite the inequality as:\n",
    "\n",
    "$$\n",
    "\\frac{\\left( \\sum_{i=1}^n \\sqrt{2a_i} \\right)^2}{\\sum_{i=1}^n \\sqrt{2b_i}} \\leq \\sum_{i=1}^n \\frac{\\sqrt{2a_i}^2}{\\sqrt{2b_i}}\n",
    "$$\n",
    "\n",
    "Now, consider the following identity:\n",
    "\n",
    "$$\n",
    "\\left( \\sum_{i=1}^n x_i \\right)^2 = \\sum_{i=1}^n x_i^2 + 2 \\sum_{1 \\leq i < j \\leq n} x_i x_j\n",
    "$$\n",
    "\n",
    "Applying this identity to the numerator, we get:\n",
    "\n",
    "$$\n",
    "\\frac{\\left( \\sum_{i=1}^n \\sqrt{2a_i} \\right)^2}{\\sum_{i=1}^n \\sqrt{2b_i}} = \\frac{\\sum_{i=1}^n (2a_i) + 2 \\sum_{1 \\leq i < j \\leq n} \\sqrt{2a_i} \\sqrt{2a_j}}{\\sum_{i=1}^n \\sqrt{2b_i}}\n",
    "$$\n",
    "\n",
    "Since $2a_i$ and $2b_i$ are even integers, $2 \\sum_{1 \\leq i < j \\leq n} \\sqrt{2a_i} \\sqrt{2a_j}$ is also even.\n",
    "\n",
    "Now, we have:\n",
    "\n",
    "$$\n",
    "\\frac{\\sum_{i=1}^n (2a_i)}{\\sum_{i=1}^n \\sqrt{2b_i}} + \\frac{2 \\sum_{1 \\leq i < j \\leq n} \\sqrt{2a_i} \\sqrt{2a_j}}{\\sum_{i=1}^n \\sqrt{2b_i}} \\leq \\sum_{i=1}^n \\frac{(2a_i)}{\\sqrt{2b_i}}\n",
    "$$\n",
    "\n",
    "Simplifying, we get:\n",
    "\n",
    "$$\n",
    "\\frac{\\sum_{i=1}^n (2a_i)}{\\sum_{i=1}^n \\sqrt{2b_i}} \\leq \\sum_{i=1}^n \\frac{(2a_i)}{\\sqrt{2b_i}}\n",
    "$$\n",
    "\n",
    "Since both sides of the inequality are non-negative, and the numerator of the left-hand side contains the terms of the denominator of the right-hand side, the inequality holds true.\n",
    "\n",
    "Therefore, Sedrakayan's Lemma is proven for $ u_i $ and $ v_i $ being square roots of even integers."
   ]
  }
 ],
 "metadata": {
  "kernelspec": {
   "display_name": "Python 3 (ipykernel)",
   "language": "python",
   "name": "python3"
  },
  "language_info": {
   "codemirror_mode": {
    "name": "ipython",
    "version": 3
   },
   "file_extension": ".py",
   "mimetype": "text/x-python",
   "name": "python",
   "nbconvert_exporter": "python",
   "pygments_lexer": "ipython3",
   "version": "3.11.7"
  }
 },
 "nbformat": 4,
 "nbformat_minor": 5
}
